analysis/Analysis.lean
@@ -3,6 +3,7 @@ import Analysis.Section_2_2
 import Analysis.Section_2_3
 import Analysis.Section_2_epilogue
 import Analysis.Section_3_1
+import Analysis.Section_3_2
 import Analysis.Section_3_3
 import Analysis.Section_3_4
 import Analysis.Section_4_1
